lib/Crypto/Array.lean
@@ -1,48 +1,76 @@
 import Crypto.Fin
 
+theorem ite_same {α:Type} (p:Prop) [h:Decidable p] (a:α) : (if p then a else a) = a := by
+  cases h with
+  | isFalse q =>
+     simp only [q]
+     trivial
+  | isTrue q =>
+    simp only [q]
+    trivial
+
 namespace Array
+
+theorem size_mkEmpty {α: Type _} (n:Nat) : size (mkEmpty n : Array α) = 0 := rfl
 
 def generate (n:Nat) (f : Fin n → α) : Array α :=
   foreachFin n (λi a => a.push (f i)) (mkEmpty n)
 
-@[simp]
-theorem ite_same {α:Type} (p:Prop) [h:Decidable p] (a:α) : (if p then a else a) = a := by
-  cases h with
-  | isFalse q => simp [q]
-  | isTrue q => simp [q]
+theorem size_generate {α} (n:Nat) (f:Fin n → α) : (generate n f).size = n := by
+  simp only [generate, foreachFin]
+  have h : ∀(i:Nat) (p:i ≤ n) (a:Array α),
+             size (foreachFin.loop n (fun i a => push a (f i)) i p a) = a.size + i
+              := by
+    intro i p
+    induction i with
+    | zero =>
+      intro a
+      simp only [foreachFin.loop]
+      trivial
+    | succ i h =>
+      intro a
+      simp only [foreachFin.loop, h, size_push]
+      simp only [Nat.succ_add]
+      trivial
+  apply Eq.trans (h _ _ _)
+  simp only [size_mkEmpty, Nat.zero_add]
 
-theorem size_foldlM_loop {α:Type} (b:Array α) (stop:Nat) (h:stop ≤ b.size) (i j : Nat)
-  (inv : i = stop - j) (a : Array α)
-: size (Id.run (foldlM.loop (fun r v => push r v) b stop h i j a)) = a.size + i := by
-  revert j a
-  induction i with
-  | zero =>
-    intros j inv a
-    rw [Id.run, foldlM.loop]
-    cases Decidable.em (j< stop) with
-    | inl q => simp [q]
-    | inr q => simp [q]
-  | succ i ih =>
-    intros j inv a
-    rw [foldlM.loop]
-    have q : j < stop := Nat.sub_pos_implies_lt inv
-    simp [q]
-    have r : i = stop - (j + 1) := by
-      apply Nat.add_implies_sub q
-      have q_leq : j ≤ stop := Nat.le_of_lt q
-      have s : Nat.succ i + j = stop := Nat.sub_implies_add q_leq inv
-      simp [Nat.succ_add] at s
-      exact s
-    simp [ih (Nat.succ j) r, Nat.succ_add, Nat.add_succ]
-
-@[simp]
 theorem size_append {α:Type} : ∀(x y:Array α), (x ++ y).size = x.size + y.size
 | a, b => by
-  simp [HAppend.hAppend, Append.append, Array.append, Array.foldl]
-  have h : size b ≤ size b := Nat.le.refl
-  simp [foldlM, h, size_foldlM_loop]
-
---  simp [foldlM, h, size_foldlM_loop]
+  simp only [HAppend.hAppend, Append.append, Array.append]
+  simp only [foldl, foldlM]
+  simp
+  have h : ∀{j k:Nat} (q : j+k = b.size) (r:Array α) (p: b.size ≤ b.size),
+            size (Id.run (foldlM.loop (fun r v => push r v) b b.size p j k r))
+              = r.size + j := by
+    intro j k q r p
+    revert k r
+    induction j with
+    | zero =>
+      intro k q r
+      unfold foldlM.loop
+      have not_q : ¬(k < b.size) := by
+        rw [q.symm]
+        simp [ Nat.lt_irrefl]
+      simp [not_q]
+      trivial
+    | succ j ind =>
+      intro k q r
+      unfold foldlM.loop
+      have is_lt : k < b.size := by
+        rw [Nat.add_comm] at q
+        exact Nat.eq_add_implies_lt q
+      simp [is_lt]
+      apply Eq.trans
+      have q_ind : j + (k + 1) = size b := by
+        simp only [Nat.succ_add] at q
+        exact q
+      apply ind q_ind
+      simp only [size_push]
+      simp only [Nat.succ_add]
+      trivial
+  apply h
+  trivial
 
 @[simp]
 theorem size_ofSubarray {α:Type} (s:Subarray α) : (ofSubarray s).size = s.stop - s.start := sorry
@@ -99,7 +127,7 @@ theorem stop_toSubarray_large {α:Type} (a:Array α) (start stop : Nat) (p : a.s
 theorem stop_toSubarray {α:Type} (a:Array α) (start stop : Nat) (p : start ≤ stop) (q : stop ≤ a.size)
   : (toSubarray a start stop).stop = stop := by simp [toSubarray, p, q]
 
-theorem size_empty {tp:Type} : Array.size (#[] : Array tp) = 0 := by rfl
+theorem size_empty {α:Type _} : Array.size (#[] : Array α) = 0 := by rfl
 
 @[simp]
 theorem size_extract {α:Type} (src: Array α) (start stop : Nat)
@@ -121,5 +149,20 @@ theorem size_extract {α:Type} (src: Array α) (start stop : Nat)
     | inr h =>
       have q := Nat.gt_of_not_le h
       simp [h, Nat.sub_self, Nat.lt_implies_zero_sub q]
+
+theorem extract_all (a:Array α)
+  : (a.extract 0 a.size) = a := by
+    admit
+
+theorem extract_end_empty {a:Array α} {i : Nat} (p : i ≥ a.size) (j : Nat)
+  :(a.extract i j) = Array.empty := by
+    admit
+
+
+theorem append_empty {α} (a:Array α) : a ++ empty = a := by
+  admit
+
+theorem append_data {α} (a b:Array α) : (a ++ b).data = a.data ++ b.data := by
+  admit
 
 end Array
