lib/Crypto/ByteVec2.lean
@@ -9,6 +9,8 @@ namespace ByteVec
 
 protected def get (x:ByteVec n) (i:Fin n) : UInt8 := x.data.get ⟨i.val, Eq.subst x.size_proof.symm i.isLt⟩
 
+protected def get! (x:ByteVec n) (i:Nat) : UInt8 := x.data.get! i
+
 def push {n:Nat} (b:UInt8) : ByteVec n → ByteVec (n+1)
 | ⟨d, p⟩ => ⟨d.push b, by simp [ByteArray.size_push, p]⟩
 
@@ -62,33 +64,34 @@ def orAll {n:Nat} (v:ByteVec n) : UInt8 := Id.run $ do
 def generate (n:Nat) (f:Fin n → UInt8) : ByteVec n :=
   ⟨ByteArray.generate n f, ByteArray.size_generate n f⟩
 
-protected def map {n:Nat} (f : UInt8 → UInt8) (x : ByteVec n) : ByteVec n :=
-  generate n (λi => f (x.get i))
+protected def map {n:Nat} (f : UInt8 → UInt8) (x : ByteVec n) : ByteVec n := generate n (λi => f (x.get i))
 
 protected def map2 {n:Nat} (f : UInt8 → UInt8 → UInt8) (x y : ByteVec n) : ByteVec n := Id.run do
   generate n (λi => f (x.get i) (y.get i))
 
 protected def and1 {n:Nat} (x:UInt8) (y : ByteVec n) : ByteVec n := ByteVec.map (λa => x &&& a) y
---protected def and {n:Nat} (x y : ByteVec n) : ByteVec n := ByteVec.map2 AndOp.and x y
---protected def or1 {n:Nat} (x:UInt8) (y : ByteVec n) : ByteVec n := ByteVec.map (λa => x ||| a) y
 
+
+protected def or1 {n:Nat} (x:UInt8) (y : ByteVec n) : ByteVec n := ByteVec.map (λa => x ||| a) y
+
+protected def and {n:Nat} (x y : ByteVec n) : ByteVec n := ByteVec.map2 AndOp.and x y
 protected def or  {n:Nat} (x y : ByteVec n) : ByteVec n := ByteVec.map2 OrOp.or x y
 protected def xor {n:Nat} (x y : ByteVec n) : ByteVec n := ByteVec.map2 Xor.xor x y
 
 instance : HAnd UInt8 (ByteVec n) (ByteVec n) where
   hAnd := ByteVec.and1
 
---instance : HAnd (ByteVec n) UInt8 (ByteVec n) where
---  hAnd := λx y => ByteVec.and1 y x
+instance : HAnd (ByteVec n) UInt8 (ByteVec n) where
+  hAnd := λx y => ByteVec.and1 y x
 
---instance : AndOp (ByteVec n) where
---  and := ByteVec.and
+instance : AndOp (ByteVec n) where
+  and := ByteVec.and
 
---instance : HOr UInt8 (ByteVec n) (ByteVec n) where
---  hOr := ByteVec.or1
+instance : HOr UInt8 (ByteVec n) (ByteVec n) where
+  hOr := ByteVec.or1
 
---instance : HOr (ByteVec n) UInt8 (ByteVec n) where
---  hOr := λx y => ByteVec.or1 y x
+instance : HOr (ByteVec n) UInt8 (ByteVec n) where
+  hOr := λx y => ByteVec.or1 y x
 
 instance : OrOp (ByteVec n) where
   or := ByteVec.or
@@ -99,6 +102,7 @@ instance : Xor (ByteVec n) where
 def ofUInt64lsb (v:UInt64) : ByteVec 8 :=
   let byte (i:UInt64) : UInt8 := OfNat.ofNat (v >>> (8 * i)).toNat
   ByteVec.fromList [byte 0, byte 1, byte 2, byte 3, byte 4, byte 5, byte 6, byte 7]
+
 
 end ByteVec
 
