lib/Crypto/List.lean
@@ -1,0 +1,8 @@
+namespace List
+
+protected
+theorem concat_to_cons (a : List α) (b:α) (c : List α)
+  : List.concat a b ++ c = a ++ b :: c := by
+    admit
+
+end List
