lib/Crypto/Vector.lean
@@ -1,0 +1,26 @@
+import Crypto.Array
+
+/--
+This module introduces arrays with an explicit type parameter for storing length.
+-/
+
+-- An array with explicit parameter for length.
+structure Vector (n:Nat) (α:Type) where
+  data : Array α
+  size_proof : data.size = n
+
+namespace Vector
+
+-- Construct a vector whose contents are generated from function.
+def generate (n:Nat) (f : Fin n → α) : Vector n α :=
+  { data := Array.generate n f,
+    size_proof := Array.size_generate n f
+  }
+
+def get {n:Nat} {α:Type _} (v:Vector n α) (i: Fin n) : α :=
+  let p : i.val < v.data.size := by
+        simp only [v.size_proof]
+        exact i.isLt
+  v.data.get ⟨i.val, p⟩
+
+end Vector
